an update

examples/Epinion/Epinions-Instrumented-5transactions.bpl
@@ -82,16 +82,61 @@ procedure {:yields} {:layer 2} process({:linear "pid"} pid:Pid, {:linear "uid"} 
 requires {:layer 2} ((pid == attPid && uid == uid0) || (pid == helperPid && uid == uid1));
 {
     var iId0 : Iid;
+	var uid2 : Uid;
+	var trust0 : int;
 	var itName0 : Itl;
+	var userName0: Unm;
     var retItemRating : [Uid]int;
 
     assume (iId0 != INIL0);
+	assume ((uid0 != uid2) && (uid1 != uid2));
 
     yield;
     call Init();
     assert  {:layer 2}   (att == false);
     assert  {:layer 2}   (hb == false);
     assert  {:layer 2}   (forall iId:Iid, uId:Uid, pid0:Pid:: hbd[iId][uId][pid0] == 0); 
+
+	yield;
+	assert {:layer 2}  (pid == attPid ==> hbd[varAtt1][varAtt2][pid] != lda);
+	assert {:layer 2}  (pid == helperPid ==> hbd[varAtt1][varAtt2][pid] != lda);	
+	assert  {:layer 2} (pid == attPid ==> !att);
+	assert  {:layer 2} (!att ==> (forall iId:Iid, uId:Uid, pid0:Pid:: hbd[iId][uId][pid0] == 0));
+
+	call UpdateTrust(uid, uid2, trust0);
+
+	assert {:layer 2}  (pid == attPid ==> hbd[varAtt1][varAtt2][pid] != lda);
+	assert {:layer 2}  (pid == helperPid ==> hbd[varAtt1][varAtt2][pid] != lda);	
+	assert  {:layer 2} (pid == attPid ==> !att);
+	assert  {:layer 2} (!att ==> (forall iId:Iid, uId:Uid, pid0:Pid:: hbd[iId][uId][pid0] == 0));
+
+	yield;
+	assert {:layer 2}  (pid == attPid ==> hbd[varAtt1][varAtt2][pid] != lda);
+	assert {:layer 2}  (pid == helperPid ==> hbd[varAtt1][varAtt2][pid] != lda);	
+	assert  {:layer 2} (pid == attPid ==> !att);
+	assert  {:layer 2} (!att ==> (forall iId:Iid, uId:Uid, pid0:Pid:: hbd[iId][uId][pid0] == 0));
+
+	call  UpdateUser(uid, userName0);
+
+	assert {:layer 2}  (pid == attPid ==> hbd[varAtt1][varAtt2][pid] != lda);
+	assert {:layer 2}  (pid == helperPid ==> hbd[varAtt1][varAtt2][pid] != lda);	
+	assert  {:layer 2} (pid == attPid ==> !att);
+	assert  {:layer 2} (!att ==> (forall iId:Iid, uId:Uid, pid0:Pid:: hbd[iId][uId][pid0] == 0));
+
+	
+	yield;
+	assert {:layer 2}  (pid == attPid ==> hbd[varAtt1][varAtt2][pid] != lda);
+	assert {:layer 2}  (pid == helperPid ==> hbd[varAtt1][varAtt2][pid] != lda);	
+	assert  {:layer 2} (pid == attPid ==> !att);
+	assert  {:layer 2} (!att ==> (forall iId:Iid, uId:Uid, pid0:Pid:: hbd[iId][uId][pid0] == 0));
+
+	call  UpdateItem(iId0, itName0);
+
+	assert {:layer 2}  (pid == attPid ==> hbd[varAtt1][varAtt2][pid] != lda);
+	assert {:layer 2}  (pid == helperPid ==> hbd[varAtt1][varAtt2][pid] != lda);	
+	assert  {:layer 2} (pid == attPid ==> !att);
+	assert  {:layer 2} (!att ==> (forall iId:Iid, uId:Uid, pid0:Pid:: hbd[iId][uId][pid0] == 0));
+   
    
     yield;
 	assert {:layer 2}  (pid == attPid ==> hbd[varAtt1][varAtt2][pid] != lda);
