examples/SimpleCurrencyExchange/SimpleCurrencyExchange-Instrumented-4transactions.bpl
@@ -1,0 +1,299 @@
+// Simple Currency Exchange Application
+// It has 4 transactions 
+// The save trade transaction is an SQL insert this why the assume must always execute together with the writes (i.e., CAS)
+
+type Pid;
+type Uid;
+type Tid;
+
+function {:builtin "MapConst"} MapConstBool(bool) : [Uid]bool;
+function {:inline} {:linear "uid"} UidCollector(x: Uid) : [Uid]bool
+{
+  MapConstBool(false)[x := true]
+}
+
+function {:builtin "MapConst"} MapConstBool2(bool) : [Tid]bool;
+function {:inline} {:linear "tid"} TidCollector(x: Tid) : [Tid]bool
+{
+  MapConstBool2(false)[x := true]
+}
+
+function {:builtin "MapConst"} MapConstBool3(bool) : [Pid]bool;
+function {:inline} {:linear "pid"} PidCollector(x: Pid) : [Pid]bool
+{
+  MapConstBool3(false)[x := true]
+}
+
+// shared variables
+var {:layer 0,2} tradeContents: [Tid][int]int;
+var {:layer 0,2} tradeUser: [Tid]Uid;
+
+// constants 
+const unique cstCurFr  :int;   // currency from
+const unique cstCurTo  :int;   // currency to
+const unique cstsAmt   :int;   // 
+const unique cstbAmt   :int;   // 
+const unique cstRate   :int;
+const unique cstTiPl   :int;
+const unique cstoCount :int;
+
+const unique NoUser : Uid;
+
+//////////////////////////////////////////////
+// Auxiliary variables for the instrumentation:
+//////////////////////////////////////////////
+
+// secondary shared variables to simulate disabled writes and reads
+
+var {:layer 0,2} copytradeContents: [Tid][int]int;
+var {:layer 0,2} copytradeUser: [Tid]Uid;
+
+var {:layer 0,2} hb : bool;
+var {:layer 0,2} att : bool;
+
+var {:layer 0,2} hbd: [Pid][int][Tid]int;  // hbd[pid][1] for the tradeUser table
+										  // hbd[pid][2] for the tradeContents table
+
+var {:layer 0,2} varAtt1 : Tid;
+
+const unique lda, sta: int;
+
+axiom ((lda == 1) && (sta == 2));
+
+const unique attPid : Pid;
+const unique helperPid : Pid;
+
+const unique tid0 : Tid;
+const unique tid1 : Tid;
+const unique tid2 : Tid;
+
+axiom ((tid0 != tid1) && (tid0 != tid2) && (tid1 != tid2));
+
+const unique TNIL0: Tid;
+
+////////////////////////////////////////////////////////////////////////////////
+// Procedure of a process
+////////////////////////////////////////////////////////////////////////////////
+	
+procedure {:yields} {:layer 2} process({:linear "pid"} pid:Pid, {:linear "uid"} uid:Uid, {:linear "tid"} tid:Tid)
+requires {:layer 2} ((pid == attPid && tid == tid0) || (pid == helperPid && tid == tid1));
+{
+
+     var cpTradeContent0     : [int]int;
+     var cpTradeUser0   : Uid;
+     var timeTrade0  : int;
+     var curFr0:int, curTo0:int, sAmt0:int, bAmt0:int, rate0:int, tiPl0:int, oCount0:int;
+
+
+    yield;
+    call Init();
+    assert  {:layer 2}   (att == false);
+    assert  {:layer 2}   (hb == false);
+    assert  {:layer 2}   (forall tid4:Tid, pid0: Pid ::  hbd[pid0][1][tid4] == 0 && hbd[pid0][2][tid4] == 0);
+   
+    yield;	
+    assert {:layer 2}  (forall tid4:Tid ::  hbd[helperPid][1][tid4] == 0 && hbd[helperPid][2][tid4] == 0);	
+    assert {:layer 2}  ( hbd[attPid][1][tid1] == 0 && hbd[attPid][2][tid1] == 0);
+	  assert  {:layer 2} (pid == attPid ==> !att);
+    assert  {:layer 2} (pid == helperPid ==> !hb);
+	  assert  {:layer 2} (!att ==> (forall tid4:Tid, pid0: Pid ::  hbd[pid0][1][tid4] == 0 && hbd[pid0][2][tid4] == 0));
+	
+	if(*)
+    {       
+		assert {:layer 2}  (forall tid4:Tid ::  hbd[helperPid][1][tid4] == 0 && hbd[helperPid][2][tid4] == 0);	
+	  assert  {:layer 2} (pid == attPid ==> !att);
+    assert  {:layer 2} (pid == helperPid ==> !hb);
+    assert {:layer 2}  ( hbd[attPid][1][tid1] == 0 && hbd[attPid][2][tid1] == 0);
+	  assert  {:layer 2} (!att ==> (forall tid4:Tid, pid0: Pid ::  hbd[pid0][1][tid4] == 0 && hbd[pid0][2][tid4] == 0));
+
+	    call SaveTrade(pid, uid,  tid, curFr0, curTo0, sAmt0, bAmt0, rate0, tiPl0, oCount0);
+		
+    assert {:layer 2}  (hbd[attPid][1][tid1] == 0 && hbd[attPid][2][tid1] == 0);
+		assert {:layer 2}  (forall tid4:Tid ::  hbd[helperPid][1][tid4] == 0 && hbd[helperPid][2][tid4] == 0);	
+    assert  {:layer 2} (pid == helperPid ==> !hb);
+	  assert  {:layer 2} (!att ==> (forall tid4:Tid, pid0: Pid ::  hbd[pid0][1][tid4] == 0 && hbd[pid0][2][tid4] == 0));
+    }
+    yield;
+    assert {:layer 2}  ( hbd[attPid][1][tid1] == 0 && hbd[attPid][2][tid1] == 0);
+    assert  {:layer 2} (pid == helperPid ==> !hb);
+    assert {:layer 2}  (forall tid4:Tid ::  hbd[helperPid][1][tid4] == 0 && hbd[helperPid][2][tid4] == 0);		
+
+	   call  cpTradeContent0 := ViewTrade(pid, uid,  tid);
+
+    assert {:layer 2}  (hbd[attPid][1][tid1] == 0 && hbd[attPid][2][tid1] == 0);
+    assert  {:layer 2} (pid == helperPid ==> !hb);
+    assert {:layer 2}  (forall tid4:Tid ::  hbd[helperPid][1][tid4] == 0 && hbd[helperPid][2][tid4] == 0);	
+    
+	
+    yield;
+    assert {:layer 2}  ( hbd[attPid][1][tid1] == 0 && hbd[attPid][2][tid1] == 0);
+    assert  {:layer 2} (pid == helperPid ==> !hb);
+    assert {:layer 2}  (forall tid4:Tid ::  hbd[helperPid][1][tid4] == 0 && hbd[helperPid][2][tid4] == 0);	
+	
+    if(*)
+    {
+      assert {:layer 2}  ( hbd[attPid][1][tid1] == 0 && hbd[attPid][2][tid1] == 0);
+      assert  {:layer 2} (pid == helperPid ==> !hb);
+      assert {:layer 2}  (forall tid4:Tid ::  hbd[helperPid][1][tid4] == 0 && hbd[helperPid][2][tid4] == 0);	
+		   
+	    call  timeTrade0 :=  GetTradeTimeStamp(pid, uid,  tid);
+      
+      assert {:layer 2}  ( hbd[attPid][1][tid1] == 0 && hbd[attPid][2][tid1] == 0);
+      assert  {:layer 2} (pid == helperPid ==> !hb);
+      assert {:layer 2}  (forall tid4:Tid ::  hbd[helperPid][1][tid4] == 0 && hbd[helperPid][2][tid4] == 0);	
+    }
+	yield;
+
+    assert {:layer 2}  ( hbd[attPid][1][tid1] == 0 && hbd[attPid][2][tid1] == 0);
+    assert  {:layer 2} (pid == helperPid ==> !hb);
+		assert {:layer 2}  (forall tid4:Tid ::  hbd[helperPid][1][tid4] == 0 && hbd[helperPid][2][tid4] == 0);	
+	
+    if(*)
+    {
+      assert {:layer 2}  ( hbd[attPid][1][tid1] == 0 && hbd[attPid][2][tid1] == 0);
+      assert  {:layer 2} (pid == helperPid ==> !hb);
+      assert {:layer 2}  (forall tid4:Tid ::  hbd[helperPid][1][tid4] == 0 && hbd[helperPid][2][tid4] == 0);		
+		   
+		call  cpTradeUser0 :=  ViewTradeUser(pid, uid,  tid);
+
+     assert {:layer 2}  (forall tid4:Tid ::  hbd[helperPid][1][tid4] == 0 && hbd[helperPid][2][tid4] == 0);		
+    }
+    yield;
+}
+
+///////////////////////////////////////////////////////////////////////////////
+/// An init procedure for initializing the auxiliary variables
+///////////////////////////////////////////////////////////////////////////////
+
+procedure  {:atomic} {:layer 2}  init()
+{
+  assume !hb;
+  assume (varAtt1 == TNIL0 && !att);
+  assume (forall tid:Tid, pid:Pid ::  hbd[pid][1][tid] == 0 && hbd[pid][2][tid] == 0) ; 
+  
+}
+  
+procedure  {:yields} {:layer 1} {:refines "init"}  Init();
+ensures {:layer 1} !hb;
+ensures {:layer 1} (varAtt1 == TNIL0 && !att);
+ensures {:layer 1} (forall tid:Tid, pid:Pid ::  hbd[pid][1][tid] == 0 && hbd[pid][2][tid] == 0) ;
+
+///////////////////////////////////////////////////////////////////////////////
+/// The instrumented SimpleCurrencyExchange transactions
+///////////////////////////////////////////////////////////////////////////////
+
+procedure {:atomic}{:layer 2}  saveTrade({:linear "pid"} pid:Pid, {:linear "uid"} uid:Uid,  {:linear "tid"} tid: Tid, curFr:int, curTo:int, sAmt:int, bAmt:int, rate:int, tiPl:int, oCount:int)
+modifies tradeUser, tradeContents;
+modifies copytradeUser, copytradeContents;
+modifies hbd, att, hb, varAtt1;
+{     
+   assume(uid != NoUser);
+   assume(tradeUser[tid] == NoUser);
+
+  if (pid == attPid && !att)
+	{ 			
+    varAtt1 := tid;	
+		att := true;
+
+    copytradeUser[tid] := uid;
+   
+    copytradeContents[tid][cstCurFr] := curFr;
+    copytradeContents[tid][cstCurTo] := curTo;
+    copytradeContents[tid][cstsAmt] := sAmt;
+    copytradeContents[tid][cstbAmt] := bAmt;
+    copytradeContents[tid][cstRate]:= rate;
+    copytradeContents[tid][cstTiPl] := tiPl;
+    copytradeContents[tid][cstoCount] := oCount;
+	}
+  else if((pid == helperPid) && !hb && att && (hbd[attPid][1][tid] >= lda || hbd[attPid][2][tid] >= lda))
+  {
+    hb := true;				
+		hbd[pid][1][tid] := sta;	
+    hbd[pid][2][tid] := sta;	
+
+    tradeUser[tid] := uid;
+   
+    tradeContents[tid][cstCurFr] := curFr;
+    tradeContents[tid][cstCurTo] := curTo;
+    tradeContents[tid][cstsAmt] := sAmt;
+    tradeContents[tid][cstbAmt] := bAmt;
+    tradeContents[tid][cstRate]:= rate;
+    tradeContents[tid][cstTiPl] := tiPl;
+    tradeContents[tid][cstoCount] := oCount;
+  }	
+	else 
+	{
+
+    tradeUser[tid] := uid;
+   
+    tradeContents[tid][cstCurFr] := curFr;
+    tradeContents[tid][cstCurTo] := curTo;
+    tradeContents[tid][cstsAmt] := sAmt;
+    tradeContents[tid][cstbAmt] := bAmt;
+    tradeContents[tid][cstRate]:= rate;
+    tradeContents[tid][cstTiPl] := tiPl;
+    tradeContents[tid][cstoCount] := oCount;
+	}
+   
+}
+procedure{:yields}{:layer 1} {:refines "saveTrade"} SaveTrade({:linear "pid"} pid:Pid, {:linear "uid"} uid:Uid, {:linear "tid"} tid: Tid, curFr:int, curTo:int, sAmt:int, bAmt:int, rate:int, tiPl:int, oCount:int);
+
+///////////////////////////////////////////////////////////////////////////////
+
+procedure {:atomic}{:layer 2} viewTrade({:linear "pid"} pid:Pid, {:linear "uid"} uid:Uid, tid: Tid) returns (cpTradeContent:[int]int)
+modifies hbd;
+{
+  assume(uid != NoUser);
+  assume(tradeUser[tid] != NoUser);
+
+  if ((pid == attPid && att) || ((pid == helperPid) && hb && att))
+	{ 			
+    hbd[pid][2][tid] := lda;		
+		cpTradeContent := tradeContents[tid];	
+	}			
+	else 
+	{
+		cpTradeContent := tradeContents[tid];
+	}
+}
+procedure {:yields}{:layer 1} {:refines "viewTrade"} ViewTrade({:linear "pid"} pid:Pid, {:linear "uid"} uid:Uid, tid: Tid) returns (cpTradeContent:[int]int);
+
+///////////////////////////////////////////////////////////////////////////////
+
+procedure {:atomic}{:layer 2} viewTradeUser({:linear "pid"} pid:Pid, {:linear "uid"} uid:Uid, tid: Tid) returns (cpTradeUser:Uid)
+modifies hbd;
+{
+  assume(uid != NoUser);
+  assume(tradeUser[tid] != NoUser);
+
+  if ((pid == attPid && att) || ((pid == helperPid) && hb && att))
+	{ 			
+    hbd[pid][1][tid] := lda;		
+		cpTradeUser := tradeUser[tid]; 			
+	}			
+	else 
+	{
+		cpTradeUser := tradeUser[tid]; 
+	}
+}
+procedure {:yields}{:layer 1} {:refines "viewTradeUser"} ViewTradeUser({:linear "pid"} pid:Pid, {:linear "uid"} uid:Uid, tid: Tid) returns (cpTradeUser:Uid);
+
+///////////////////////////////////////////////////////////////////////////////
+
+procedure {:atomic}{:layer 2} getTradeTimeStamp({:linear "pid"} pid:Pid, {:linear "uid"} uid:Uid, tid: Tid) returns (timeTrade:int)
+modifies hbd;
+{
+  assume(uid != NoUser);
+  assume(tradeUser[tid] != NoUser);
+
+  if ((pid == attPid && att) || ((pid == helperPid) && hb && att))
+	{ 			
+    hbd[pid][2][tid] := lda;		
+		timeTrade:=tradeContents[tid][cstTiPl]; 			
+	}			
+	else 
+	{
+		timeTrade:=tradeContents[tid][cstTiPl]; 
+	} 
+}
+procedure {:yields}{:layer 1} {:refines "getTradeTimeStamp"} GetTradeTimeStamp({:linear "pid"} pid:Pid, {:linear "uid"} uid:Uid, tid: Tid) returns (timeTrade:int);
