examples/FusionTicket/FusionTicket-Instrumented-PC-5transactions.bpl
@@ -4,7 +4,7 @@
 // Non-robustness check between CC and PC
 // RUN: /usr/bin/time -v --format="%e" %boogie -noinfer -typeEncoding:m -tracePOs -traceTimes  -trace  -useArrayTheory "%s" > "%t"
 // RUN: %diff "%s.expect" "%t"
-// 0.70
+// 0.73
 
 type Pid;
 type Eid;   // Event identifier type
@@ -58,8 +58,10 @@ requires {:layer 2} (pid == attPid || pid == helperPid);
 
      var venueId0:Vid, venueId1:Vid, eventId0:Eid, eventId1:Eid;
      var eventsId0     : [Eid]bool;
+	 var eventsId1     : [Eid]bool;
      var evNbTicket0   : int;
      var ticketPrice0  : int;
+	 var ticketPrice1  : int;
 
 	assume (eventId1 != eventId0);
     assume (eventId0 != ENIL0 && venueId0 != VNIL0 && eventId1 != ENIL0 && venueId1 != VNIL0);
@@ -78,7 +80,7 @@ requires {:layer 2} (pid == attPid || pid == helperPid);
 	assert  {:layer 2} (!att ==> (forall venueId:Vid, eventId:Eid:: hbd[1][venueId][eventId] == 0 &&  
 									hbd[2][venueId][eventId] == 0));
 	
-	if(pid == attPid)
+	if(*)
     {       
 		assert {:layer 2}  (pid == attPid ==> hbd[2][varAtt1][varAtt2] != lda);
 	    assert {:layer 2}  (pid == helperPid ==> hbd[2][varAtt1][varAtt2] != lda);		
@@ -106,17 +108,46 @@ requires {:layer 2} (pid == attPid || pid == helperPid);
 	   assert {:layer 2}  (pid == attPid ==> hbd[2][varAtt1][varAtt2] != lda);
 	   assert {:layer 2}  (pid == helperPid ==> hbd[2][varAtt1][varAtt2] != lda);	           
     }
+	yield;
+	assert {:layer 2}  (pid == attPid ==> hbd[2][varAtt1][varAtt2] != lda);
+	assert {:layer 2}  (pid == helperPid ==> hbd[2][varAtt1][varAtt2] != lda);	
+	
+	
+    if(*)
+    {       
+	   assert {:layer 2}  (pid == attPid ==> hbd[2][varAtt1][varAtt2] != lda);
+	   assert {:layer 2}  (pid == helperPid ==> hbd[2][varAtt1][varAtt2] != lda);	
+
+	   call  ticketPrice1 := PurchaseTicket(pid,eventId0,venueId0);
+
+	   assert {:layer 2}  (pid == attPid ==> hbd[2][varAtt1][varAtt2] != lda);
+	   assert {:layer 2}  (pid == helperPid ==> hbd[2][varAtt1][varAtt2] != lda);	           
+    }
 	
     yield;
 		assert {:layer 2}  (pid == attPid ==> hbd[2][varAtt1][varAtt2] != lda);
 	    assert {:layer 2}  (pid == helperPid ==> hbd[2][varAtt1][varAtt2] != lda);		
 	
-    if(pid == helperPid)
+    if(*)
     {
 		assert {:layer 2}  (pid == attPid ==> hbd[2][varAtt1][varAtt2] != lda);
 	    assert {:layer 2}  (pid == helperPid ==> hbd[2][varAtt1][varAtt2] != lda);		
 		   
 	    call  eventsId0 :=  Browse(pid,venueId0);
+
+        assert {:layer 2}  (pid == attPid ==> hbd[2][varAtt1][varAtt2] != lda);
+	    assert {:layer 2}  (pid == helperPid ==> hbd[2][varAtt1][varAtt2] != lda);	
+    }
+	yield;
+		assert {:layer 2}  (pid == attPid ==> hbd[2][varAtt1][varAtt2] != lda);
+	    assert {:layer 2}  (pid == helperPid ==> hbd[2][varAtt1][varAtt2] != lda);		
+	
+    if(*)
+    {
+		assert {:layer 2}  (pid == attPid ==> hbd[2][varAtt1][varAtt2] != lda);
+	    assert {:layer 2}  (pid == helperPid ==> hbd[2][varAtt1][varAtt2] != lda);		
+		   
+		call  eventsId1 :=  Browse(pid,venueId1);
 
         assert {:layer 2}  (pid == attPid ==> hbd[2][varAtt1][varAtt2] != lda);
 	    assert {:layer 2}  (pid == helperPid ==> hbd[2][varAtt1][varAtt2] != lda);	
